compiler/printing/typeDecToPPScript.sml
@@ -77,14 +77,14 @@ Definition mk_pps_for_type_def:
 End
 
 Definition mk_pp_type_def:
-  mk_pp_type fixes (funs : type_def) = Dletrec unknown_loc (MAP (mk_pps_for_type fixes) funs)
+  mk_pp_type fixes (funs : type_def) = Dletrec NoLocs (MAP (mk_pps_for_type fixes) funs)
 End
 
 Definition mk_pp_tabbrev_def:
   mk_pp_tabbrev fixes tvars nm ast_t =
   let body = FOLDR (\nm exp. Fun (pppre nm) exp) (pp_of_ast_t fixes ast_t) tvars in
     (* eta-expansion to avoid value restriction violations *)
-    Dlet unknown_loc (Pvar (pppre nm)) (Fun «x» (App Opapp [body; Var (Short «x»)]))
+    Dlet NoLocs (Pvar (pppre nm)) (Fun «x» (App Opapp [body; Var (Short «x»)]))
 End
 
 Definition pps_for_dec_def:
