basis/Word8ArrayProgScript.sml
@@ -10,7 +10,7 @@ Libs
 val _ = translation_extends "Word8Prog";
 
 val _ = ml_prog_update (add_dec
-  ``Dtabbrev unknown_loc [] «byte_array» (Atapp [] (Short «word8array»))`` I);
+  ``Dtabbrev NoLocs [] «byte_array» (Atapp [] (Short «word8array»))`` I);
 
 val _ = ml_prog_update (open_module "Word8Array");
 
@@ -18,17 +18,17 @@ val _ = append_decs
    ``[mk_binop «array» Aw8alloc;
       mk_binop «sub» Aw8sub;
       mk_unop «length» Aw8length;
-      Dlet unknown_loc (Pvar «update») (Fun «x» (Fun «y» (Fun «z»
+      Dlet NoLocs (Pvar «update») (Fun «x» (Fun «y» (Fun «z»
         (App Aw8update [Var (Short «x»); Var (Short «y»); Var (Short «z»)]))));
-      Dlet unknown_loc (Pvar «copy»)
+      Dlet NoLocs (Pvar «copy»)
         (Fun «src» (Fun «srcoff» (Fun «len» (Fun «dst» (Fun «dstoff»
         (App CopyAw8Aw8 [Var (Short «src»);Var (Short «srcoff»);Var (Short «len»);
                          Var (Short «dst»);Var (Short «dstoff»)]))))));
-      Dlet unknown_loc (Pvar «copyVec»)
+      Dlet NoLocs (Pvar «copyVec»)
         (Fun «src» (Fun «srcoff» (Fun «len» (Fun «dst» (Fun «dstoff»
         (App CopyStrAw8 [Var (Short «src»);Var (Short «srcoff»);Var (Short «len»);
                          Var (Short «dst»);Var (Short «dstoff»)]))))));
-      Dlet unknown_loc (Pvar «substring»)
+      Dlet NoLocs (Pvar «substring»)
         (Fun «src» (Fun «srcoff» (Fun «len»
         (App CopyAw8Str [Var (Short «src»);Var (Short «srcoff»);Var (Short «len»)]))))]``;
 
