basis/mlbasicsProgScript.sml
@@ -14,12 +14,12 @@ Libs
 val _ = translation_extends"StringProg"
 
 Definition mk_binop_def:
-  mk_binop name prim = Dlet unknown_loc (Pvar name)
+  mk_binop name prim = Dlet NoLocs (Pvar name)
     (Fun «x» (Fun «y» (App prim [Var (Short «x»); Var (Short «y»)])))
 End
 
 Definition mk_unop_def:
-  mk_unop name prim = Dlet unknown_loc (Pvar name)
+  mk_unop name prim = Dlet NoLocs (Pvar name)
     (Fun «x» (App prim [Var (Short «x»)]))
 End
 
@@ -27,15 +27,15 @@ End
 (* list, bool, and option come from the primitive types in
  * semantics/primTypesTheory *)
 val _ = append_prog
-  ``[Tdec (Dtabbrev unknown_loc [] "int" (Tapp [] TC_int));
-     Tdec (Dtabbrev unknown_loc [] "unit" (Tapp [] TC_tup));
-     Tdec (Dtabbrev unknown_loc [] "string" (Tapp [] TC_string));
-     Tdec (Dtabbrev unknown_loc ["'a"] "ref" (Tapp [Tvar "'a"] TC_ref));
-     Tdec (Dtabbrev unknown_loc ["'a"] "vector" (Tapp [Tvar "'a"] TC_vector));
-     Tdec (Dtabbrev unknown_loc ["'a"] "array" (Tapp [Tvar "'a"] TC_array));
-     Tdec (Dtabbrev unknown_loc [] "exn" (Tapp [] TC_exn));
-     Tdec (Dtabbrev unknown_loc [] "word" (Tapp [] TC_word64));
-     Tdec (Dtabbrev unknown_loc [] "char" (Tapp [] TC_char))]``
+  ``[Tdec (Dtabbrev NoLocs [] "int" (Tapp [] TC_int));
+     Tdec (Dtabbrev NoLocs [] "unit" (Tapp [] TC_tup));
+     Tdec (Dtabbrev NoLocs [] "string" (Tapp [] TC_string));
+     Tdec (Dtabbrev NoLocs ["'a"] "ref" (Tapp [Tvar "'a"] TC_ref));
+     Tdec (Dtabbrev NoLocs ["'a"] "vector" (Tapp [Tvar "'a"] TC_vector));
+     Tdec (Dtabbrev NoLocs ["'a"] "array" (Tapp [Tvar "'a"] TC_array));
+     Tdec (Dtabbrev NoLocs [] "exn" (Tapp [] TC_exn));
+     Tdec (Dtabbrev NoLocs [] "word" (Tapp [] TC_word64));
+     Tdec (Dtabbrev NoLocs [] "char" (Tapp [] TC_char))]``
 *)
 
 val _ = trans "+" intSyntax.plus_tm;
