translator/ml_progLib.sml
@@ -332,8 +332,8 @@ fun ML_code_upd nm mp_thm adjs (ML_code code) = let
 
 (* --- *)
 
-val unknown_loc = locationTheory.unknown_loc_def |> concl |> dest_eq |> fst;
-val loc = unknown_loc;
+val no_locs = prim_mk_const {Name = "NoLocs", Thy = "ast"};
+val loc = no_locs;
 
 val init_state =
   ML_code ([SPEC_ALL init_state_def],[init_env_def],[],ML_code_NIL);
@@ -382,7 +382,7 @@ fun add_Dtype loc tds_tm = ML_code_upd "add_Dtype"
                 APPEND,namespaceTheory.mk_id_def])]
 
 (*
-val loc = unknown_loc
+val loc = no_locs
 val n_tm = ``"bar"``
 val l_tm = ``[]:ast_t list``
 *)
@@ -400,7 +400,7 @@ fun add_Dtabbrev loc l1_tm l2_tm l3_tm = ML_code_upd "add_Dtabbrev"
 fun add_Dlet eval_thm var_str = let
     val (_, eval_thm_xs) = strip_comb (concl eval_thm)
     val mp_thm = ML_code_Dlet_var |> SPECL (tl eval_thm_xs
-        @ [mlstringSyntax.mk_mlstring var_str,unknown_loc])
+        @ [mlstringSyntax.mk_mlstring var_str,no_locs])
   in ML_code_upd "add_Dlet" mp_thm
     [solve_ml_imp_mp eval_thm,
      solve_ml_imp_conv (SIMP_CONV bool_ss []
