compiler/parsing/README.md
@@ -38,7 +38,7 @@ OCaml lexer and parser frontend for the Candle theorem prover.
 
 [pegexec_cml_foScript.sml](pegexec_cml_foScript.sml):
 First-order PEG exec instantiated to CakeML surface types:
-  input: (token # locs) list
+  input: (token # location$locs) list
   values: mlptree list  (as in cmlPEG)
   errors: string
   rule keys: MMLnonT inf
